\documentclass{article}
\usepackage[utf8]{inputenc}
\usepackage{setspace}
\usepackage{amssymb}
\usepackage{amsmath}
\usepackage{amsthm}
\usepackage{systeme}
\usepackage{mathtools}
\usepackage{hyperref}

\def\R{\mathbb{R}}
\def\rank{\text{rank}}
\def\proj{\text{proj}}
\DeclareMathOperator{\im}{im}

\begin{document}

\section{Problem 1}

\subsection{Question a}

~

\begin{equation*}
    \begin{split}
        &\begin{cases}
            v_1=(0,1,1)\\
            v_2=(1,1,1)\\
            v_3=(1,-2,2)\\
        \end{cases}\\
        u_1=&v_1=(0,1,1)\\
        u_2=&v_2-\proj_{u_1}v_2\\
        =&(1,1,1)-\frac{\langle(1,1,1),(0,1,1)\rangle}{\langle(0,1,1),(0,1,1)\rangle}(0,1,1)\\
        =&(1,1,1)-(0,1,1)\\
        =&(1,0,0)\\
        u_3=&v_3-\proj_{u_1}v_3-\proj_{u_2}v_3\\
        =&(1,-2,2)-\frac{\langle(1,-2,2),(0,1,1)\rangle}{\langle(0,1,1),(0,1,1)\rangle}(0,1,1)-\frac{\langle(1,-2,2),(1,0,0)\rangle}{\langle(1,0,0),(1,0,0)\rangle}(1,0,0)\\
        =&(1,-2,2)-(0,0,0)-(1,0,0)\\
        =&(0,-2,2)\\
        e_1=&\frac{u_1}{\|u_1\|}\\
        =&(0,\frac{\sqrt{2}}{2},\frac{\sqrt{2}}{2})\\
        e_2=&\frac{u_2}{\|u_2\|}\\
        =&(1,0,0)\\
        e_3=&\frac{u_3}{\|u_3\|}\\
        =&(0,-\frac{\sqrt{2}}{2},\frac{\sqrt{2}}{2})\\
        \Rightarrow&\overline{\beta}=\{(0,\frac{\sqrt{2}}{2},\frac{\sqrt{2}}{2}),(1,0,0),(0,-\frac{\sqrt{2}}{2},\frac{\sqrt{2}}{2})\}\\
    \end{split}
\end{equation*}

\subsection{Question b}

~

\begin{equation*}
    \begin{split}
        &\begin{cases}
            v_1=1+x^2\\
            v_2=-1+x\\
            v_3=1+x\\
        \end{cases}\\
        u_1=&v_1=1+x^2\\
        u_2=&v_2-\proj_{u_1}v_2\\
        =&-1+x-\frac{\langle-1+x,1+x^2\rangle}{\langle1+x^2,1+x^2\rangle}1+x^2\\
        =&-1+x+\frac{5}{16}(1+x^2)\\
        =&-\frac{11}{16}+x+\frac{5}{16}x^2\\
        u_3=&v_3-\proj_{u_1}v_3-\proj_{u_2}v_3\\
        =&1+x-\frac{\langle1+x,1+x^2\rangle}{\langle1+x^2,1+x^2\rangle}(1+x^2)-\frac{\langle1+x,-\frac{11}{16}+x+\frac{5}{16}x^2\rangle}{\langle-\frac{11}{16}+x+\frac{5}{16}x^2,-\frac{11}{16}+x+\frac{5}{16}x^2\rangle}(-\frac{11}{16}+x+\frac{5}{16}x^2)\\
        =&-\frac{38}{203}+\frac{32}{29}x-\frac{220}{203}x^2\\
        e_1=&\frac{u_1}{\|u_1\|}\\
        =&\frac{\sqrt{15}}{2\sqrt{7}}+\frac{\sqrt{15}}{2\sqrt{7}}x^2\\
        e_2=&\frac{u_2}{\|u_2\|}\\
        =&-\frac{11\sqrt{3}}{2\sqrt{29}}+\frac{8\sqrt{3}}{\sqrt{29}}x+\frac{5\sqrt{3}}{2\sqrt{29}}x^2\\
        e_3=&\frac{u_3}{\|u_3\|}\\
        =&-\frac{19\sqrt{3}}{\sqrt{203}}+\frac{16\sqrt{21}}{\sqrt{29}}x-\frac{110\sqrt{3}}{\sqrt{203}}x^2\\
        \Rightarrow&\overline{\beta}=\{\frac{\sqrt{15}}{2\sqrt{7}}+\frac{\sqrt{15}}{2\sqrt{7}}x^2,-\frac{11\sqrt{3}}{2\sqrt{29}}+\frac{8\sqrt{3}}{\sqrt{29}}x+\frac{5\sqrt{3}}{2\sqrt{29}}x^2,-\frac{19\sqrt{3}}{\sqrt{203}}+\frac{16\sqrt{21}}{\sqrt{29}}x-\frac{110\sqrt{3}}{\sqrt{203}}x^2\}\\
    \end{split}
\end{equation*}

\newpage

\section{Problem 2}

\subsection{Question a}

~

\begin{equation*}
    \begin{split}
        &x\coloneqq(x_1,x_2,x_3,x_4)\\
        &\begin{cases}
            \langle x,(1,0,1,2)\rangle =0\\
            \langle x,(1,-1,0,1)\rangle=0\\
        \end{cases}\\
        \Rightarrow&\begin{cases}
            x_1+x_3+2x_4=0\\
            x_1-x_2+x_4=0\\
        \end{cases}\\
        \Rightarrow&\begin{cases}
            x_1=x_1\\
            x_2=x_1+x_4\\
            x_3=-x_1-2x_4\\
            x_4=x_4
        \end{cases}\\
        \Rightarrow& W^\perp=\text{Span}\{(1,1,-1,0),(0,1,-2,1)\}\\
    \end{split}
\end{equation*}

\begin{equation*}
    \begin{split}
        &W:\\
        u_1&=v_1=(1,0,1,2)\\
        u_2&=v_2-\proj_{u_1}v_2\\
        &=(1,-1,0,1)-\frac{\langle(1,-1,0,1),(1,0,1,2)\rangle}{\langle(1,0,1,2),(1,0,1,2)\rangle}(1,0,1,2)\\
        &=(1,-1,0,1)-\frac{1}{2}(1,0,1,2)\\
        &=(\frac{1}{2},-1,-\frac{1}{2},0)\\
        e_1&=\frac{u_1}{\|u_1\|}\\
        &=(\frac{1}{\sqrt{6}},0,\frac{1}{\sqrt{6}},\frac{2}{\sqrt{6}})\\
        e_2&=\frac{u_2}{\|u_2\|}\\
        &=(\frac{1}{\sqrt{6}},-\frac{2}{\sqrt{6}},-\frac{1}{\sqrt{6}},0)\\
        &\Rightarrow\text{Orthonormal basis for }W:\{(\frac{1}{\sqrt{6}},0,\frac{1}{\sqrt{6}},\frac{2}{\sqrt{6}}),(\frac{1}{\sqrt{6}},-\frac{2}{\sqrt{6}},-\frac{1}{\sqrt{6}},0)\}\\
    \end{split}
\end{equation*}

\begin{equation*}
    \begin{split}
        &W^\perp:\\
        u_1&=v_1=(1,1,-1,0)\\
        u_2&=v_2-\proj_{u_1}v_2\\
        &=(0,1,-2,1)-\frac{\langle(0,1,-2,1),(1,1,-1,0)\rangle}{\langle(1,1,-1,0),(1,1,-1,0)\rangle}(1,1,-1,0)\\
        &=(0,1,-2,1)-(1,1,-1,0)\\
        &=(-1,0,-1,1)\\
        e_1&=\frac{u_1}{\|u_1\|}\\
        &=(\frac{1}{\sqrt{3}},\frac{1}{\sqrt{3}},-\frac{1}{\sqrt{3}},0)\\
        e_2&=\frac{u_2}{\|u_2\|}\\
        &=(-\frac{1}{\sqrt{3}},0,-\frac{1}{\sqrt{3}},\frac{1}{\sqrt{3}})\\
        &\Rightarrow\text{Orthonormal basis for }W^\perp:\{(\frac{1}{\sqrt{3}},\frac{1}{\sqrt{3}},-\frac{1}{\sqrt{3}},0),(-\frac{1}{\sqrt{3}},0,-\frac{1}{\sqrt{3}},\frac{1}{\sqrt{3}})\}\\
    \end{split}
\end{equation*}

\subsection{Question b}

~

\begin{equation*}
    \begin{split}
        &w_1\coloneqq a(\frac{1}{\sqrt{6}},0,\frac{1}{\sqrt{6}},\frac{2}{\sqrt{6}})+b(\frac{1}{\sqrt{6}},-\frac{2}{\sqrt{6}},-\frac{1}{\sqrt{6}},0)\\
        &w_2\coloneqq c(\frac{1}{\sqrt{3}},\frac{1}{\sqrt{3}},-\frac{1}{\sqrt{3}},0)+d(-\frac{1}{\sqrt{3}},0,-\frac{1}{\sqrt{3}},\frac{1}{\sqrt{3}})\\
        &w_1+w_2=(1,1,1,1)\\
        \Rightarrow&\begin{cases}
            \frac{1}{\sqrt{6}}a+\frac{1}{\sqrt{6}}b+\frac{1}{\sqrt{3}}c-\frac{1}{\sqrt{3}}d=1\\
            -\frac{2}{\sqrt{6}}b+\frac{1}{\sqrt{3}}c=1\\
            \frac{1}{\sqrt{6}}a-\frac{1}{\sqrt{6}}b-\frac{1}{\sqrt{3}}c-\frac{1}{\sqrt{3}}d=1\\
            \frac{2}{\sqrt{6}}a+\frac{1}{\sqrt{3}}d=1\\
        \end{cases}\\
        \Rightarrow&\begin{cases}
            a=\frac{4}{\sqrt{6}}\\
            b=-\frac{2}{\sqrt{6}}\\
            c=\frac{1}{\sqrt{3}}\\
            d=-\frac{1}{\sqrt{3}}\\
        \end{cases}\\
        \Rightarrow&\begin{cases}
            w_1=(\frac{1}{3},\frac{2}{3},1,\frac{4}{3})\\
            w_2=(\frac{2}{3},\frac{1}{3},0,-\frac{1}{3})\\
        \end{cases}
    \end{split}
\end{equation*}

\newpage

\section{Problem 3}

\subsection{Question a}

~

\begin{equation*}
    \begin{split}
        &u\in W\\
        \Rightarrow&\langle u,v\rangle=0\forall v\in W^\perp\\
        &\langle v, w\rangle=0\forall w\in{W^\perp}^\perp\\
        \Rightarrow&W\subseteq {W^\perp}^\perp\\
        &\text{Let }W \text{ be a subspace over }V \text{ with dimension }n\\
        &\dim(W)+\dim(W^\perp)=n\\
        &\dim(W^\perp)+\dim({W^\perp}^\perp)=n\\
        \Rightarrow&\dim(W)+\dim(W^\perp)=\dim(W^\perp)+\dim({W^\perp}^\perp)\\
        \Rightarrow&\dim(W)=\dim({W^\perp}^\perp)\\
        \Rightarrow&W={W^\perp}^\perp\\
    \end{split}
\end{equation*}

\subsection{Question b}

~

\subsubsection*{$(W_1+W_2)^\perp\subseteq {W_1}^\perp\cap {W_2}^\perp$}

~

\begin{equation*}
    \begin{split}
        &v\in (W_1+W_2)^\perp\\
        \Rightarrow&\langle v,w_1+w_2\rangle=0\forall w_1\in W_1\land w_2\in W_2\\
        &\text{Let } w_1=0:\\
        &\langle v,w_2\rangle=0\implies v\in {W_2}^\perp\\
        &\text{Similarly } v\in {W_1}^\perp\\
        \Rightarrow&v\in{W_1}^\perp\cap {W_2}^\perp\\
        \Rightarrow&(W_1+W_2)^\perp\subseteq {W_1}^\perp\cap {W_2}^\perp\\
    \end{split}
\end{equation*}

\subsubsection*{${W_1}^\perp\cap {W_2}^\perp\subseteq (W_1+W_2)^\perp$}

~

\begin{equation*}
    \begin{split}
        &v\in{W_1}^\perp\cap {W_2}^\perp\\
        \Rightarrow&\langle v,w_1\rangle=0\land \langle v,w_2\rangle=0\forall w_1\in W_1\land w_2\in W_2\\
        \Rightarrow&\langle v,w_1\rangle+\langle v,w_2\rangle =0\\
        \Rightarrow&\langle v,w_1+w_2\rangle=0\\
        \Rightarrow&v\in (W_1+W_2)^\perp\\
        \Rightarrow&{W_1}^\perp\cap {W_2}^\perp\subseteq (W_1+W_2)^\perp\\
        &(W_1+W_2)^\perp\subseteq {W_1}^\perp\cap {W_2}^\perp\land{W_1}^\perp\cap {W_2}^\perp\subseteq (W_1+W_2)^\perp\\
        \Rightarrow&(W_1+W_2)^\perp= {W_1}^\perp\cap {W_2}^\perp\\
    \end{split}
\end{equation*}

\subsection{Question c}

~

\begin{equation*}
    \begin{split}
        &(W_1\cap W_2)^\perp\\
        =&({W_1^\perp}^\perp\cap{W_2^\perp}^\perp)^\perp\\
        =&((W_1^\perp+W_2^\perp)^\perp)^\perp\\
        =&W_1^\perp+W_2^\perp\\
        \Rightarrow&(W_1\cap W_2)^\perp=W_1^\perp+W_2^\perp\\
    \end{split}
\end{equation*}

\newpage

\section{Problem 4}

\subsection{Question a}

~

\begin{equation*}
    \begin{split}
        &v=\sum^n_{i=1}c_iv_i\\
        \Rightarrow&\langle v,v_i\rangle=\langle\sum^n_{i=1}c_iv_i,v_i\rangle=c_i\langle v_i,v_i\rangle\leftarrow v_i\perp v_j\forall i\ne j\in \R\\
        \Rightarrow&c_i=\frac{\langle v,v_i\rangle}{\|v_i\|^2}\\
        &\langle v,v\rangle=\langle\sum^n_{i=1}c_iv_i,\sum^n_{i=1}c_iv_i\rangle\\
        =&\sum_{i=1}^n{c_i}^2\|v_i\|^2\\
        =&\sum_{i=1}^n\frac{\langle v,v_i\rangle^2}{\|v_i\|^2}\\
        =&\|v\|^2\\
        &\|v_i\|^2=1\leftarrow \beta\text{ is orthonormal}\\
        \Rightarrow&\|v\|=\sqrt{\sum_{i=1}^n\langle v,v_i\rangle^2}\\
    \end{split}
\end{equation*}

\subsection{Question b}

~

\begin{equation*}
    \begin{split}
        &u=\sum^n_{i=1}d_iv_i\\
        \Rightarrow&d_i=\frac{\langle u,v_i\rangle}{\|v_i\|^2}\\
        &\langle u,v\rangle=\langle\sum^n_{i=1}d_iv_i\sum^n_{i=1}c_iv_i\rangle\\
        =&\sum^n_{i=1}c_id_i\|v_i\|^2\\
        =&\sum^n_{i=1}\langle v,v_i\rangle\langle u,v_i\rangle\leftarrow \|v_i\|^2=1\\
        \Rightarrow&\langle u,v\rangle=\sum^n_{i=1}\langle v,v_i\rangle\langle u,v_i\rangle\\
    \end{split}
\end{equation*}

\newpage

\section{Problem 5}

\subsection{Question a}

~

\begin{equation*}
    \begin{split}
        &v=\sum^n_{i=1}c_iv_i\\
        \Rightarrow&\langle v,v_i\rangle=\langle\sum^n_{i=1}c_iv_i,v_i\rangle=c_i\langle v_i,v_i\rangle\leftarrow v_i\perp v_j\forall i\ne j\in \R\\
        \Rightarrow&c_i=\frac{\langle v,v_i\rangle}{\|v_i\|^2}\\
        &\|v_1\|^2=1\\
        \Rightarrow&c_i=\langle v,v_i\rangle\\
        \Rightarrow&v=\sum^n_{i=1}\langle v,v_i\rangle v_i\\
        \Rightarrow&f(v)=f(\sum^n_{i=1}\langle v,v_i\rangle v_i)\\
        &f\text{ is a linear transformation}\\
        \Rightarrow&f(v)=\sum^n_{i=1}\langle v,v_i\rangle f(v_i)\\
        \Rightarrow&f(v)=\langle v,\sum^n_{i=1}f(v_i)v_i\rangle=\langle v,w\rangle\\
        \Rightarrow&w=\sum^n_{i=1}f(v_i)v_i\\
        &w\text{ is unique because }v_i\text{ are orthonormal, there cannnot be another way to form }w\text{ of the same value}\\
    \end{split}
\end{equation*}

\subsection{Question b}

~

\begin{equation*}
    \begin{split}
        &\langle p(x),g(x)\rangle=p(0)g(0)+p(1)g(1)+p(2)g(2)\\
        &f(p(x))=\int^1_{-1}p(x)\\
        &\beta=\{1,x,x^2\}\\
        &u_1=v_1=1\\
        &u_2=v_2-\proj_{u_1}v_2\\
        =&x-\frac{\langle x,1\rangle}{\langle1,1\rangle}1\\
        =&-1+x\\
        &u_3=v_3-\proj_{u_1}v_3-\proj_{u_2}v_3\\
        =&x^2-\frac{5}{3}-2(x-1)\\
        =&\frac{1}{3}-2x+x^2\\
        &e_1=\frac{u_1}{\|u_1\|}\\
        =&\frac{1}{\sqrt{3}}\\
        &e_2=\frac{u_2}{\|u_2\|}\\
        =&-\frac{1}{\sqrt{2}}+\frac{1}{\sqrt{2}}x\\
        &e_3=\frac{u_3}{\|u_3\|}\\
        =&\frac{\sqrt{6}}{6}-\sqrt{6}x+\frac{\sqrt{6}}{2}x^2\\
        \Rightarrow&\beta'=\{\frac{1}{\sqrt{3}},-\frac{1}{\sqrt{2}}+\frac{1}{\sqrt{2}}x,\frac{\sqrt{6}}{6}-\sqrt{6}x+\frac{\sqrt{6}}{2}x^2\}=\{v_1,v_2,v_3\}\\
        &g(x)=\sum^3_{i=1}f(v_i)v_i\\
        =&\frac{1}{3}\int_{-1}^{1}\frac{1}{3}dx+\int_{-1}^{1}-\frac{1}{\sqrt{2}}+\frac{1}{\sqrt{2}}xdx(-\frac{1}{\sqrt{2}}+\frac{1}{\sqrt{2}}x)+\int_{-1}^{1}\frac{\sqrt{6}}{6}-\sqrt{6}x+\frac{\sqrt{6}}{2}x^2dx(\frac{\sqrt{6}}{6}-\sqrt{6}x+\frac{\sqrt{6}}{2}x^2)\\
        =&\frac{2}{9}-\sqrt{2}(-\frac{1}{\sqrt{2}}+\frac{1}{\sqrt{2}}x)+2\sqrt{\frac{2}{3}}(\frac{\sqrt{6}}{6}-\sqrt{6}x+\frac{\sqrt{6}}{2}x^2)\\
        =&\frac{17}{9}-5x+2x^2\\
        \Rightarrow&g(x)=\frac{17}{9}-5x+2x^2\\
    \end{split}
\end{equation*}

\newpage

\section{Reference}

~

Jeffery Shu

~

Frank Zhu


\end{document}